Cleanup up to definition of machine strategy.

theories/OGS/Game.v
@@ -6,8 +6,12 @@ The OGS Game (§ 5.1 and 5.2)
 From OGS Require Import Prelude.
 From OGS.Utils Require Import Rel.
 From OGS.Ctx Require Import All Ctx.
-From OGS.OGS Require Import Subst Obs Machine.
-From OGS.ITree Require Import Event ITree Eq Delay Structure Properties Guarded.
+From OGS.OGS Require Import Obs.
+From OGS.ITree Require Import Event ITree.
+
+Reserved Notation "↓⁺ Ψ" (at level 9).
+Reserved Notation "↓⁻ Ψ" (at level 9).
+Reserved Notation "↓[ p ] Ψ" (at level 9).
 
 (*|
 Games (§ 5.1)
@@ -62,61 +66,54 @@ OGS Games (§ 5.2)
 ==================
 |*)
 
+Variant polarity : Type := Act | Pas .
+Derive NoConfusion for polarity.
+
+Equations p_switch : polarity -> polarity :=
+  p_switch Act := Pas ;
+  p_switch Pas := Act .
+#[global] Notation "p ^" := (p_switch p) (at level 5).
+
 Section with_param.
 (*|
 We consider an observation structure.
 |*)
   Context `{CC : context T C} {obs : obs_struct T C}.
 
-  Inductive pctx (Δ : C) : ctx C -> Type :=
-  | PCemp : pctx Δ (∅ ▶ Δ)
-  | PCcat {Ψ Γ} (xs : pctx Δ Ψ) (i : Ψ ∋ Γ) (E : C) : pctx Δ (Ψ ▶ E)
-  .
-
-  Equations prefix {X} (Γ : ctx X) {x} : Γ ∋ x -> ctx X :=
-    prefix (Γ ▶ _) top     := Γ ;
-    prefix (Γ ▶ _) (pop i) := prefix Γ i .
-
-  Equations view 
-
-  Equations r_prefix {X} {Γ : ctx X} {x} (i : Γ ∋ x) : prefix Γ i ⊆ Γ :=
-    r_prefix top     _ j := pop j ;
-    r_prefix (pop i) _ j := pop (r_prefix i _ j) .
-
-  Equations view {Δ Ψ} : pctx Δ Ψ -> ctx C :=
-    view (PCemp)        := (∅ ▶ Δ) ;
-    view (PCcat xs i E) := view (prefix ) .
+  Definition ogs_ctx := ctx C.
 
 (*|
 Interleaved contexts (Def 5.12)
-Collapsing functions (Def 5.13, see Utils/Ctx.v for auxiliary definitions)
+Collapsing functions (Def 5.13)
 |*)
-  Definition alt_ext : Type := ctx (context).
-  Notation "↓⁺ a" := (join_even a) (at level 9).
-  Notation "↓⁻ a" := (join_odd a) (at level 9).
-  Notation "↓[ b ] a" := (join_even_odd_aux b a) (at level 9).
+  Equations join_pol : polarity -> ogs_ctx -> C :=
+    join_pol Act ∅ₓ       := ∅ ;
+    join_pol Act (Ψ ▶ₓ Γ) := join_pol Pas Ψ +▶ Γ ;
+    join_pol Pas ∅ₓ       := ∅ ;
+    join_pol Pas (Ψ ▶ₓ Γ) := join_pol Act Ψ .
+
+  Notation "↓⁺ Ψ" := (join_pol Act Ψ).
+  Notation "↓⁻ Ψ" := (join_pol Pas Ψ).
+  Notation "↓[ p ] Ψ" := (join_pol p Ψ).
 
 (*|
 Half games and games (Def 5.15)
 |*)
-  Definition ogs_hg : half_game alt_ext alt_ext :=
-    {| g_move := fun es => obs∙ ↓⁺es ;
-       g_next := fun es m => (es ▶ dom∙ m) |} .
+  Definition ogs_hg : half_game ogs_ctx ogs_ctx :=
+    {| g_move Ψ := obs∙ ↓⁺Ψ ;
+       g_next Ψ m := Ψ ▶ₓ m_dom m |} .
 
-  Definition ogs_g : game alt_ext alt_ext :=
+  Definition ogs_g : game ogs_ctx ogs_ctx :=
     {| g_client := ogs_hg ;
        g_server := ogs_hg  |} .
 
-  Definition ogs_e : event alt_ext alt_ext := e_of_g ogs_g.
+  Definition ogs_e : event ogs_ctx ogs_ctx := e_of_g ogs_g.
 
-  Definition ogs_act (Δ : context) : psh alt_ext := itree ogs_e (fun _ => obs∙ Δ).
-  Definition ogs_pas (Δ : context) : psh alt_ext := h_pasv ogs_hg (ogs_act Δ).
+  Definition ogs_act (Δ : C) : psh ogs_ctx := itree ogs_e (fun _ => obs∙ Δ).
+  Definition ogs_pas (Δ : C) : psh ogs_ctx := h_pasv ogs_hg (ogs_act Δ).
 
-End withFam.
+End with_param.
 
-Notation "↓⁺ a" := (join_even a) (at level 9).
-Notation "↓⁻ a" := (join_odd a) (at level 9).
-Notation "↓[ b ] a" := (join_even_odd_aux b a) (at level 9).
-Notation "Ⓟ" := true.
-Notation "Ⓞ" := false.
-
+#[global] Notation "↓⁺ Ψ" := (join_pol Act Ψ).
+#[global] Notation "↓⁻ Ψ" := (join_pol Pas Ψ).
+#[global] Notation "↓[ p ] Ψ" := (join_pol p Ψ).
